zoo/common/countable: [solve_countable]: Support (non-recursive) indexed inductive types.

theories/zoo/common/countable.v
@@ -3,165 +3,327 @@ From stdpp Require Export
 
 From zoo Require Import
   prelude.
-From zoo.ltac2 Require Import
+From zoo.ltac2 Require
   Array
   Constr
   Control
-  Env
+  Ind
   List
-  Option
-  Std
   String
   Notations.
 From zoo Require Import
   options.
 
-#[local] Ltac2 error msg :=
-  let msg := String.app "error: " msg in
-  Control.throw_invalid_argument msg.
+Module solve_countable.
+  Import Ltac2.Init.
+  Import Ltac2.Notations.
 
-#[local] Ltac2 prod () :=
-  match Env.expand [@prod] with
-  | IndRef ind :: _ =>
-      ind
-  | _ =>
-      error "cannot find [prod]"
-  end.
-#[local] Ltac2 pair () :=
-  match Env.expand [@pair] with
-  | ref_ :: _ =>
-      ref_
-  | _ =>
-      error "cannot find [pair]"
-  end.
-#[local] Ltac2 unit () :=
-  match Env.expand [@unit] with
-  | ref_ :: _ =>
-      Constr.Unsafe.make_app (Env.instantiate ref_) Array.empty
-  | _ =>
-      error "cannot find [unit]"
-  end.
-#[local] Ltac2 tt () :=
-  match Env.expand [@tt] with
-  | ref_ :: _ =>
-      Constr.Unsafe.make_app (Env.instantiate ref_) Array.empty
-  | _ =>
-      error "cannot find [tt]"
-  end.
+  Ltac2 Type error :=
+    [ Goal_invalid
+    | Type_not_inductive
+    | Type_empty
+    | Internal_error
+    ].
 
-#[local] Ltac2 rec parameters constr :=
-  match Constr.Unsafe.kind constr with
-  | Constr.Unsafe.Prod bdr constr =>
-      let param := Constr.Binder.type bdr in
-      param :: parameters constr
-  | _ =>
-      []
-  end.
-#[local] Ltac2 record_fields data inst :=
-  let ctor := Constr.Unsafe.make_constructor (Ind.get_constructor data 0) inst in
-  parameters (Constr.type ctor).
+  Ltac2 error_to_string err :=
+    match err with
+    | Goal_invalid  =>
+        "invalid goal"
+    | Type_not_inductive =>
+        "not an inductive type"
+    | Type_empty =>
+        "empty inductive type"
+    | Internal_error =>
+        "internal error"
+    end.
+  Ltac2 error err :=
+    let err := error_to_string err in
+    let err := String.app "solve_countable: " err in
+    Control.throw_invalid_argument err.
 
-#[local] Ltac2 solve_countable_0 rcd ind data inst :=
-  let flds := record_fields data inst in
-  let num_fld := List.length flds in
-  let prod := prod () in
-  let pair := pair () in
-  let unit := unit () in
-  let tt := tt () in
-  let tpl :=
-    List.fold_right (fun fld acc =>
-      Constr.Unsafe.make_app
-        (Env.instantiate (IndRef prod))
-        [|fld; acc|]
-    ) flds unit
-  in
-  let encode :=
-    Constr.Unsafe.make_lambda
-      (Constr.Binder.make None rcd)
-      ( Constr.Unsafe.make_case_simple
-        ind
-        rcd
-        tpl
-        (Constr.Unsafe.make_rel 1)
-        ( List.fold_right
-          ( fun fld acc =>
-            Constr.Unsafe.make_lambda
-              (Constr.Binder.make None fld)
-              acc
-          )
-          flds
-          ( List.fold_righti (fun i fld acc =>
-              Constr.Unsafe.make_app
-                (Env.instantiate pair)
-                [|fld
-                ; '_
-                ; Constr.Unsafe.make_rel (Int.sub num_fld i)
-                ; acc
-                |]
-            ) flds tt
-          )
+  Ltac2 Type info :=
+    { info_type : constr ;
+      info_inductive : inductive ;
+      info_data : Ind.data ;
+      info_instance : instance ;
+      info_indices : constr array ;
+      info_number_constructor : int ;
+      info_constructors : constructor array ;
+      info_fieldss : constr array array ;
+      info_sum_inductive : inductive ;
+      info_prod_inductive : inductive ;
+    }.
+
+  Ltac2 info_constructor info i :=
+    Array.get (info.(info_constructors)) i.
+  Ltac2 info_constructor_constr info i :=
+    let ctor := info_constructor info i in
+    Constr.Unsafe.make_constructor ctor (info.(info_instance)).
+  Ltac2 info_fields info i :=
+    Array.get (info.(info_fieldss)) i.
+  Ltac2 info_arity info i :=
+    Array.length (info_fields info i).
+
+  Ltac2 info ty :=
+    let (ind, indices) := Constr.head_tail ty in
+    let (ind, inst) :=
+      match Constr.Unsafe.kind ind with
+      | Constr.Unsafe.Ind ind inst =>
+          ind, inst
+      | _ =>
+          error Type_not_inductive
+      end
+    in
+    let data := Ind.data ind in
+    let num_ctor := Ind.nconstructors data in
+    if Int.equal num_ctor 0 then
+      error Type_empty
+    else
+      let ctors :=
+        Array.init num_ctor (fun i =>
+          Ind.get_constructor data i
         )
-      )
-  in
-  let decode :=
-    Constr.Unsafe.make_lambda
-      (Constr.Binder.make None tpl)
-      ( fst (List.fold_right
-        ( fun fld acc =>
-          let ty :=
+      in
+      let fldss :=
+        Array.map (fun ctor =>
+          let ctor :=
             Constr.Unsafe.make_app
-              (Env.instantiate (IndRef prod))
-              [|fld; snd acc|]
+              (Constr.Unsafe.make_constructor ctor inst)
+              indices
           in
-          ( Constr.Unsafe.make_case_simple
-              prod
-              ty
-              rcd
-              (Constr.Unsafe.make_rel 1)
-              ( Constr.Unsafe.make_lambdas
-                [ Constr.Binder.make None fld
-                ; Constr.Binder.make None (snd acc)
-                ]
-                (fst acc)
-              )
-          , ty
-          )
-        )
-        flds
-        ( Constr.Unsafe.make_app'
-          ( Constr.Unsafe.make_constructor
-            (Ind.get_constructor data 0)
-            inst
-          )
-          ( List.mapi (fun i _fld =>
-              Constr.Unsafe.make_rel (Int.mul 2 (Int.sub num_fld i))
-            ) flds
-          )
-        , unit
-        )
-      ))
-  in
-  refine (
-    Constr.Unsafe.make_app
-      '@inj_countable'
-      [|'_; '_; '_; '_; '_; encode; decode; '_|]
-  ) ;
-  Control.focus 1 2 (fun () => apply _);
-  solve [intros []; auto].
-#[local] Ltac2 solve_countable_1 rcd :=
-  match Constr.Unsafe.kind rcd with
-  | Constr.Unsafe.Ind ind inst =>
-      let data := Ind.data ind in
-      if Bool.neg (Int.equal 1 (Ind.nconstructors data)) then
-        error "not a record type"
-      else
-        solve_countable_0 rcd ind data inst
-  | _ =>
-      Control.throw (Invalid_argument (Some (Message.of_constr rcd)))
-  end.
-#[local] Ltac2 solve_countable () :=
-  match! goal with [|- Countable ?rcd] =>
-    solve_countable_1 rcd
-  end.
+          let ctor_ty := Constr.type ctor in
+          let flds := Constr.product_parameters ctor_ty in
+          Array.of_list flds
+        ) ctors
+      in
+      let sum_ind :=
+        match Constr.Unsafe.kind '@sum with
+        | Constr.Unsafe.Ind ind _ =>
+            ind
+        | _ =>
+            error Internal_error
+        end
+      in
+      let prod_ind :=
+        match Constr.Unsafe.kind '@prod with
+        | Constr.Unsafe.Ind ind _ =>
+            ind
+        | _ =>
+            error Internal_error
+        end
+      in
+      { info_type := ty ;
+        info_inductive := ind ;
+        info_data := data ;
+        info_instance := inst ;
+        info_indices := indices ;
+        info_number_constructor := num_ctor ;
+        info_constructors := ctors ;
+        info_fieldss := fldss ;
+        info_sum_inductive := sum_ind ;
+        info_prod_inductive := prod_ind ;
+      }.
+
+  Ltac2 encode_branch info i :=
+    let flds := info_fields info i in
+    let num_fld := Array.length flds in
+    let bdrs :=
+      Array.map (fun fld =>
+        Constr.Binder.make None fld
+      ) flds
+    in
+    let bdrs := Array.to_list bdrs in
+    let body :=
+      List.init_foldl (fun acc i =>
+        let fld := Constr.Unsafe.make_rel (Int.sub num_fld i) in
+        Constr.Unsafe.make_app
+          '@pair
+          [|'_; '_; acc; fld|]
+      ) 'tt num_fld
+    in
+    let body :=
+      let ty := if Int.equal i 0 then 'unit else '_ in
+      Constr.Unsafe.make_app
+        '@inr
+        [|ty; '_; body|]
+    in
+    let body :=
+      List.init_foldl (fun acc _ =>
+        Constr.Unsafe.make_app
+          '@inl
+          [|'_; '_; acc|]
+      ) body (Int.sub (Int.sub (info.(info_number_constructor)) i) 1)
+    in
+    Constr.Unsafe.make_lambdas bdrs body.
+  Ltac2 encode_case info :=
+    Constr.Unsafe.make_case_simple
+      (info.(info_inductive))
+      (info.(info_type))
+      '_
+      (Constr.Unsafe.make_rel 1)
+      ( Array.init
+          (info.(info_number_constructor))
+          (encode_branch info)
+      ).
+  Ltac2 encode info :=
+    Constr.Unsafe.make_lambda
+      (Constr.Binder.make None (info.(info_type)))
+      (encode_case info).
+
+  Ltac2 extract_arguments_2 ty :=
+    match Constr.Unsafe.kind ty with
+    | Constr.Unsafe.App _ tys =>
+        if Bool.neg (Int.equal (Array.length tys) 2) then
+          error Internal_error
+        else
+          Array.get tys 0, Array.get tys 1
+    | _ =>
+        error Internal_error
+    end.
+  Ltac2 rec decode_branch' info i j ty' :=
+    if Int.equal j 0 then
+      Constr.Unsafe.make_app
+        '@Some
+        [|info.(info_type)
+        ; Constr.Unsafe.make_app
+            (info_constructor_constr info i)
+            ( Array.append
+                (info.(info_indices))
+                ( Array.init (info_arity info i) (fun j =>
+                    Constr.Unsafe.make_rel (Int.add (Int.mul 2 j) 1)
+                  )
+                )
+            )
+        |]
+    else
+      let ty := info.(info_type) in
+      let (ty'_1, ty'_2) := extract_arguments_2 ty' in
+      (* for some reason, we have to reconstruct [ty'], otherwise we might get an exception [Constr.DestKO] *)
+      let ty' := Constr.Unsafe.make_app '@prod [|ty'_1; ty'_2|] in
+      Constr.Unsafe.make_case_simple
+        (info.(info_prod_inductive))
+        ty'
+        '(option $ty)
+        (Constr.Unsafe.make_rel 2)
+        [|Constr.Unsafe.make_lambdas
+            [ Constr.Binder.make None ty'_1
+            ; Constr.Binder.make None ty'_2
+            ]
+            (decode_branch' info i (Int.sub j 1) ty'_1)
+        |].
+  Ltac2 decode_branch info i ty' :=
+    Constr.Unsafe.make_lambda
+      (Constr.Binder.make None ty')
+      ( Constr.Unsafe.make_let
+          (Constr.Binder.make None 'unit)
+          'tt
+          (decode_branch' info i (info_arity info i) ty')
+      ).
+  Ltac2 rec decode_case' info i ty' :=
+    let ty := info.(info_type) in
+    if Int.equal i (-1) then
+      '(@None $ty)
+    else
+      let (ty'_l, ty'_r) := extract_arguments_2 ty' in
+      (* for some reason, we have to reconstruct [ty'], otherwise we might get an exception [Constr.DestKO] *)
+      let ty' := Constr.Unsafe.make_app '@sum [|ty'_l; ty'_r|] in
+      Constr.Unsafe.make_case_simple
+        (info.(info_sum_inductive))
+        ty'
+        '(option $ty)
+        (Constr.Unsafe.make_rel 1)
+        [|Constr.Unsafe.make_lambda
+            (Constr.Binder.make None ty'_l)
+            (decode_case' info (Int.sub i 1) ty'_l)
+        ; decode_branch info i ty'_r
+        |].
+  Ltac2 decode_case info ty' :=
+    decode_case'
+      info
+      (Int.sub (info.(info_number_constructor)) 1)
+      ty'.
+  Ltac2 decode info ty' :=
+    Constr.Unsafe.make_lambda
+      (Constr.Binder.make None ty')
+      (decode_case info ty').
+
+  Ltac2 main' info :=
+    let encode := encode info in
+    let ty' := Constr.product_result (Constr.type encode) in
+    let decode := decode info ty' in
+    let _ := Constr.type decode in
+    refine (
+      Constr.Unsafe.make_app
+        '@inj_countable
+        [|'_; '_; '_; '_; '_; encode; decode; '_|]
+    ) ;
+    Control.focus 1 2 (fun () => apply _);
+    solve [intros []; auto].
+  Ltac2 main () :=
+    lazy_match! goal with
+    | [|- Countable ?ty] =>
+        main' (info ty)
+    | [|- _] =>
+        error Goal_invalid
+    end.
+End solve_countable.
+
 Ltac solve_countable :=
-  ltac2:(solve_countable ()).
+  ltac2:(solve_countable.main ()).
+
+Module tests.
+  Record test_1 := {
+    test_1_1 : nat ;
+  }.
+  #[local] Instance test_1_eq_dec : EqDecision test_1 :=
+    ltac:(solve_decision).
+  #[local] Instance test_1_countable :
+    Countable test_1.
+  Proof.
+    solve_countable.
+  Qed.
+
+  Record test_2 A1 A2 A3 := {
+    test_2_1 : A1 ;
+    test_2_2 : A2 ;
+    test_2_3 : A3 ;
+  }.
+  #[local] Instance test_2_eq_dec `{!EqDecision A1, !EqDecision A2, !EqDecision A3} : EqDecision (test_2 A1 A2 A3) :=
+    ltac:(solve_decision).
+  #[local] Instance test_2_countable `{Countable A1, Countable A2, Countable A3} :
+    Countable (test_2 A1 A2 A3).
+  Proof.
+    solve_countable.
+  Qed.
+
+  Inductive test_3 :=
+    | Test31 : test_3
+    | Test32 : nat → test_3
+    | Test33 : nat → bool → test_3.
+  #[local] Instance test_3_eq_dec : EqDecision test_3 :=
+    ltac:(solve_decision).
+  #[local] Instance test_3_countable :
+    Countable test_3.
+  Proof.
+    solve_countable.
+  Qed.
+
+  Inductive test_4 A1 A2 A3 :=
+    | Test41 : test_4 A1 A2 A3
+    | Test42 : nat → test_4 A1 A2 A3
+    | Test43 : nat → bool → test_4 A1 A2 A3
+    | Test44 : A1 → test_4 A1 A2 A3
+    | Test45 : A2 → test_4 A1 A2 A3
+    | Test46 : A3 → test_4 A1 A2 A3
+    | Test47 : A1 → A2 → test_4 A1 A2 A3
+    | Test48 : A1 → A3 → test_4 A1 A2 A3
+    | Test49 : A2 → A3 → test_4 A1 A2 A3
+    | Test410 : A1 → A2 → A3 → test_4 A1 A2 A3.
+  #[local] Instance test_4_eq_dec `{!EqDecision A1, !EqDecision A2, !EqDecision A3} : EqDecision (test_4 A1 A2 A3) :=
+    ltac:(solve_decision).
+  #[local] Instance test_4_countable `{Countable A1, Countable A2, Countable A3} :
+    Countable (test_4 A1 A2 A3).
+  Proof.
+    solve_countable.
+  Qed.
+End tests.
