theories/zoo/ltac2/Array.v
@@ -6,3 +6,9 @@ From zoo Require Import
   prelude.
 From zoo Require Import
   options.
+
+Ltac2 foldr :=
+  fold_right.
+
+Ltac2 foldl :=
+  fold_left.
