theories/zoo/ltac2/Constr.v
@@ -19,59 +19,113 @@ Module Unsafe.
     make (Var id).
   Ltac2 make_meta meta :=
     make (Meta meta).
-  Ltac2 make_evar evar constrs :=
-    make (Evar evar constrs).
+  Ltac2 make_evar evar ts :=
+    make (Evar evar ts).
   Ltac2 make_sort sort :=
     make (Sort sort).
-  Ltac2 make_cast constr cast ty :=
-    make (Cast constr cast ty).
-  Ltac2 make_prod bdr constr :=
-    make (Prod bdr constr).
-  Ltac2 make_lambda bdr constr :=
-    make (Lambda bdr constr).
-  Ltac2 make_let bdr constr1 constr2 :=
-    make (LetIn bdr constr1 constr2).
-  Ltac2 make_app constr constrs :=
-    make (App constr constrs).
+  Ltac2 make_cast t cast ty :=
+    make (Cast t cast ty).
+  Ltac2 make_prod bdr t :=
+    make (Prod bdr t).
+  Ltac2 make_lambda bdr t :=
+    make (Lambda bdr t).
+  Ltac2 make_let bdr t1 t2 :=
+    make (LetIn bdr t1 t2).
+  Ltac2 make_app t ts :=
+    make (App t ts).
   Ltac2 make_constant const inst :=
     make (Constant const inst).
   Ltac2 make_ind ind inst :=
     make (Ind ind inst).
   Ltac2 make_constructor ctor inst :=
     make (Constructor ctor inst).
-  Ltac2 make_case case info inv constr brs :=
-    make (Case case info inv constr brs).
-  Ltac2 make_fix structs i bdrs constrs :=
-    make (Fix structs i bdrs constrs).
-  Ltac2 make_cofix i bdrs constrs :=
-    make (CoFix i bdrs constrs).
-  Ltac2 make_proj proj relevance constr :=
-    make (Proj proj relevance constr).
+  Ltac2 make_case case info inv t brs :=
+    make (Case case info inv t brs).
+  Ltac2 make_fix structs i bdrs ts :=
+    make (Fix structs i bdrs ts).
+  Ltac2 make_cofix i bdrs ts :=
+    make (CoFix i bdrs ts).
+  Ltac2 make_proj proj relevance t :=
+    make (Proj proj relevance t).
   Ltac2 make_uint63 n :=
     make (Uint63 n).
   Ltac2 make_float f :=
     make (Float f).
   Ltac2 make_string str :=
     make (String str).
-  Ltac2 make_array inst constrs constr1 constr2 :=
-    make (Array inst constrs constr1 constr2).
+  Ltac2 make_array inst ts t1 t2 :=
+    make (Array inst ts t1 t2).
 
-  Ltac2 make_lambdas bdrs constr :=
-    List.fold_right make_lambda bdrs constr.
+  Ltac2 make_lambdas bdrs t :=
+    List.fold_right make_lambda bdrs t.
 
-  Ltac2 make_app' constr constrs :=
-    make_app constr (Array.of_list constrs).
+  Ltac2 make_app' t ts :=
+    make_app t (Array.of_list ts).
 
-  Ltac2 make_case_simple ind ty1 ty2 constr br :=
+  Ltac2 make_case_simple ind ty1 ty2 t brs :=
     make_case
       (case ind)
-      ( ( Constr.Unsafe.make_lambda
-          (Constr.Binder.make None ty1)
+      ( ( make_lambda
+          (Binder.make None ty1)
           ty2
         ),
-        Constr.Binder.Relevant
+        Binder.Relevant
       )
-      Constr.Unsafe.NoInvert
-      constr
-      (Array.make 1 br).
+      NoInvert
+      t
+      brs.
 End Unsafe.
+
+Ltac2 rec head t :=
+  match Unsafe.kind t with
+  | Unsafe.App t _ =>
+      head t
+  | _ =>
+      t
+  end.
+
+#[local] Ltac2 rec head_tail' t acc :=
+  match Unsafe.kind t with
+  | Unsafe.App t ts =>
+      let acc := Array.append ts acc in
+      head_tail' t acc
+  | _ =>
+      t, acc
+  end.
+Ltac2 head_tail t :=
+  head_tail' t Array.empty.
+
+Ltac2 tail t :=
+  let (_, tl) := head_tail t in
+  tl.
+
+Ltac2 rec product_arity t :=
+  match Unsafe.kind t with
+  | Unsafe.Prod _ t =>
+      Int.add (product_arity t) 1
+  | _ =>
+      0
+  end.
+
+#[local] Ltac2 rec product_decompose' t acc :=
+  match Unsafe.kind t with
+  | Unsafe.Prod bdr t =>
+      let ty := Binder.type bdr in
+      product_decompose' t (ty :: acc)
+  | _ =>
+      List.rev acc, t
+  end.
+Ltac2 product_decompose t :=
+  product_decompose' t [].
+
+Ltac2 product_parameters t :=
+  let (params, _) := product_decompose t in
+  params.
+
+Ltac2 rec product_result t :=
+  match Unsafe.kind t with
+  | Unsafe.Prod _ t =>
+      product_result t
+  | _ =>
+      t
+  end.
