theories/zoo/ltac2/Constructor.v
@@ -1,0 +1,20 @@
+From Ltac2 Require Export
+  Constructor
+  Init.
+
+From zoo Require Import
+  prelude.
+From zoo.ltac2 Require Import
+  Constr
+  Ind.
+From zoo Require Import
+  options.
+
+Ltac2 number_index t inst :=
+  Ind.number_index (inductive t) inst.
+
+Ltac2 arity_full t inst :=
+  let t := Constr.Unsafe.make_constructor t inst in
+  Constr.product_arity (Constr.type t).
+Ltac2 arity t inst :=
+  Int.sub (arity_full t inst) (number_index t inst).
