theories/zoo/ltac2/Ind.v
@@ -1,0 +1,17 @@
+From Ltac2 Require Export
+  Ind
+  Init.
+
+From zoo Require Import
+  prelude.
+From zoo.ltac2 Require Import
+  Constr.
+From zoo Require Import
+  options.
+
+Ltac2 nconstructors' t :=
+  nconstructors (data t).
+
+Ltac2 number_index t inst :=
+  let t := Constr.Unsafe.make_ind t inst in
+  Constr.product_arity (Constr.type t).
