theories/zoo/ltac2/List.v
@@ -7,7 +7,18 @@ From zoo Require Import
 From zoo Require Import
   options.
 
-Ltac2 fold_righti fn xs acc :=
+#[local] Ltac2 rec init_foldl' fn acc i n :=
+  if Int.equal n 0 then
+    acc
+  else
+    let acc := fn acc i in
+    init_foldl' fn acc (Int.add i 1) (Int.sub n 1).
+Ltac2 init_foldl fn acc :=
+  init_foldl' fn acc 0.
+
+Ltac2 foldr :=
+  fold_right.
+Ltac2 foldri fn xs acc :=
   let rec go i xs acc :=
     match xs with
     | [] =>
@@ -17,3 +28,8 @@ Ltac2 fold_righti fn xs acc :=
     end
   in
   go 0 xs acc.
+
+Ltac2 foldl :=
+  fold_left.
+Ltac2 foldli:=
+  fold_lefti.
